Decouple from CeTA

Superposition_Calculus/Ground_Critical_Pairs.thy
@@ -1,14 +1,24 @@
 theory Ground_Critical_Pairs
-  imports TRS.Trs
+  imports
+    "Abstract-Rewriting.Relative_Rewriting"
+    First_Order_Terms.Term
+    Knuth_Bendix_Order.Subterm_and_Context
 begin
 
-definition ground_critical_pairs :: "('f, 'v) trs \<Rightarrow> ('f, 'v) rule set" where
+definition vars_rewrite_rule where
+  "vars_rewrite_rule r = vars_term (fst r) \<union> vars_term (snd r)"
+
+definition rewrite_steps where
+  "rewrite_steps R = {(ctxt\<langle>t\<^sub>1\<rangle>, ctxt\<langle>t\<^sub>2\<rangle>) | ctxt t\<^sub>1 t\<^sub>2. (t\<^sub>1, t\<^sub>2) \<in> R}"
+
+definition ground_critical_pairs :: "('f, 'v) term rel \<Rightarrow> ('f, 'v) term rel" where
   "ground_critical_pairs R = {(ctxt\<langle>r\<^sub>2\<rangle>, r\<^sub>1) | ctxt l r\<^sub>1 r\<^sub>2. (ctxt\<langle>l\<rangle>, r\<^sub>1) \<in> R \<and> (l, r\<^sub>2) \<in> R}"
 
 locale ground_critical_pair_lemma =
   fixes dummy_fun :: 'f and dummy_var :: 'v
   assumes
-    WCR_iff_ground_critical_pairs_subset_join_rstep: "\<And>(R :: ('f, 'v) trs).
-      vars_trs R = {} \<Longrightarrow> WCR (rstep R) \<longleftrightarrow> ground_critical_pairs R \<subseteq> (rstep R)\<^sup>\<down>"
+    WCR_iff_ground_critical_pairs_subset_join_rewrite_steps: "\<And>(R :: ('f, 'v) term rel).
+      (\<Union>r \<in> R. vars_rewrite_rule r) = {} \<Longrightarrow>
+      WCR (rewrite_steps R) \<longleftrightarrow> ground_critical_pairs R \<subseteq> (rewrite_steps R)\<^sup>\<down>"
 
 end
