Superposition_Calculus/CeTA_Term_Rewriting.thy
@@ -1,0 +1,13 @@
+(*
+Author:  Christian Sternagel <c.sternagel@gmail.com>
+Author:  René Thiemann <rene.thiemann@uibk.ac.at>
+License: LGPL (see file COPYING.LESSER)
+*)
+chapter \<open>Term Rewriting\<close>
+
+theory CeTA_Term_Rewriting
+  imports
+    Knuth_Bendix_Order.Subterm_and_Context
+begin
+
+end
