Superposition_Calculus/Ground_Critical_Pairs_String_Vars.thy
@@ -1,6 +1,6 @@
 theory Ground_Critical_Pairs_String_Vars
   imports
-    CR.Critical_Pairs
+    TRS.Trs
     Ground_Critical_Pairs
 begin
 
@@ -10,7 +10,7 @@ lemma ballI2: "(\<And>x y. (x, y) \<in> A \<Longrightarrow> P x y) \<Longrightar
 abbreviation is_ground_trm where
   "is_ground_trm t \<equiv> vars_term t = {}"
 
-lemma mem_ground_critical_pairs_if_mem_critical_pairs:
+(* lemma mem_ground_critical_pairs_if_mem_critical_pairs:
   fixes s t :: "('f, string) term"
   assumes
     ground_R: "\<forall>(s, t) \<in> R. is_ground_trm s \<and> is_ground_trm t" and
@@ -115,23 +115,316 @@ proof -
   qed
 qed
 
-lemma ground_critical_pair_lemma:
+lemma foo:
+  assumes ground_R: "\<forall>(s, t) \<in> R. is_ground_trm s \<and> is_ground_trm t"
+  shows "\<And>r. r \<in> rewrite_steps R \<Longrightarrow> r \<in> rstep R"
+    by (smt (verit, del_insts) mem_Collect_eq rewrite_steps_def rstep_ctxt subset_iff subset_rstep) *)
+
+lemma converse_rewrite_step: "(rewrite_steps R)\<inverse> = rewrite_steps (R\<inverse>)"
+  by (auto simp: rewrite_steps_def)
+
+lemma subset_rewrite_steps: "R \<subseteq> rewrite_steps R"
+  apply (rule Set.subsetI)
+  unfolding rewrite_steps_def mem_Collect_eq
+  by (metis ctxt_apply_term.simps(1) prod.exhaust)
+
+lemma ground_critical_pairs_fork:
+  assumes cp: "(l, r) \<in> ground_critical_pairs R"
+  shows "(r, l) \<in> (rewrite_steps R)\<inverse> O rewrite_steps R"
+proof -
+  from cp [unfolded ground_critical_pairs_def, simplified]
+  obtain ctxt t r\<^sub>1 t' where "l = ctxt\<langle>t'\<rangle>" and "(ctxt\<langle>t\<rangle>, r) \<in> R" and "(t, t') \<in> R"
+    by metis
+    
+  have "(r, ctxt\<langle>t\<rangle>) \<in> (rewrite_steps R)\<inverse>"
+    using \<open>(ctxt\<langle>t\<rangle>, r) \<in> R\<close> subset_rewrite_steps by blast
+  moreover have "(ctxt\<langle>t\<rangle>, l) \<in> rewrite_steps R"
+    using \<open>(t, t') \<in> R\<close> \<open>l = ctxt\<langle>t'\<rangle>\<close> rewrite_steps_def by fast
+  ultimately show ?thesis by auto
+qed
+
+lemma ground_critical_pairs_complete:
+  fixes R :: "('f, string) trs"
+  assumes cp: "(l, r) \<in> ground_critical_pairs R"
+    and no_join: "(l, r) \<notin> (rewrite_steps R)\<^sup>\<down>"
+  shows "\<not> WCR (rewrite_steps R)"
+proof (rule notI)
+  assume wcr: "WCR (rewrite_steps R)"
+  moreover from ground_critical_pairs_fork[OF cp] obtain u where
+    ul: "(u, l) \<in> rewrite_steps R" and ur: "(u, r) \<in> rewrite_steps R"
+    by auto
+  ultimately show False
+    using no_join
+    unfolding WCR_on_def
+    by simp
+qed
+
+
+
+lemma rewrite_steps_closed_ctxt:
+  assumes "(s, t) \<in> (rewrite_steps R)\<^sup>*"
+  shows "(C\<langle>s\<rangle>, C\<langle>t\<rangle>) \<in> (rewrite_steps R)\<^sup>*"
+proof -
+  from assms obtain n where "(s,t) \<in> (rewrite_steps R)^^n"
+    using rtrancl_is_UN_relpow by auto
+  then show ?thesis
+  proof (induct n arbitrary: s)
+    case 0 then show ?case by auto
+  next
+    case (Suc n)
+    from relpow_Suc_D2[OF \<open>(s,t) \<in> (rewrite_steps R)^^Suc n\<close>] obtain u
+      where "(s,u) \<in> (rewrite_steps R)" and "(u,t) \<in> (rewrite_steps R)^^n" by auto
+    from \<open>(s,u) \<in> (rewrite_steps R)\<close> have "(C\<langle>s\<rangle>,C\<langle>u\<rangle>) \<in> (rewrite_steps R)"
+      apply (simp add: rewrite_steps_def)
+      using ctxt_ctxt by blast
+    from Suc and \<open>(u,t) \<in> (rewrite_steps R)^^n\<close> have "(C\<langle>u\<rangle>,C\<langle>t\<rangle>) \<in> (rewrite_steps R)\<^sup>*" by simp
+    with \<open>(C\<langle>s\<rangle>,C\<langle>u\<rangle>) \<in> (rewrite_steps R)\<close> show ?case by auto
+ qed
+qed
+
+
+lemma critical_pairs_main:
   fixes R :: "('f, string) trs"
   assumes ground_R: "\<forall>(s, t) \<in> R. is_ground_trm s \<and> is_ground_trm t"
-  shows "WCR (rstep R) \<longleftrightarrow> (\<forall> (s, t) \<in> ground_critical_pairs R. (s, t) \<in> (rstep R)\<^sup>\<down>)"
-  unfolding critical_pair_lemma
+  assumes st1: "(s, t1) \<in> rewrite_steps R" and st2: "(s, t2) \<in> rewrite_steps R"
+  shows "(t1, t2) \<in> join (rewrite_steps R) \<or>
+    (\<exists> ctxt l r. t1 = ctxt\<langle>l\<rangle> \<and> t2 = ctxt\<langle>r\<rangle> \<and>
+      ((l, r) \<in> ground_critical_pairs R \<or> (r, l) \<in> ground_critical_pairs R))"
+proof -
+  let ?R = "rewrite_steps R"
+  let ?CP = "ground_critical_pairs R"
+  from st1 obtain C1 l1 r1 where
+    lr1: "(l1, r1) \<in> R" and s1: "s = C1\<langle>l1\<rangle>" and t1: "t1 = C1\<langle>r1\<rangle>"
+    by (auto simp: rewrite_steps_def)
+  from st2 obtain C2 l2 r2 where
+    lr2: "(l2, r2) \<in> R" and s2: "s = C2\<langle>l2\<rangle>" and t2: "t2 = C2\<langle>r2\<rangle>"
+    by (auto simp: rewrite_steps_def)
+  from s1 s2 have id: "C1\<langle>l1\<rangle> = C2\<langle>l2\<rangle>"
+    by simp
+  let ?q = "\<lambda>s t. (s, t) \<in> join ?R \<or> (\<exists>C l r. s = C\<langle>l\<rangle> \<and> t = C\<langle>r\<rangle> \<and> ((l, r) \<in> ?CP \<or> (r, l) \<in> ?CP))"
+  let ?p = "\<lambda>(C1, C2). \<forall>l1 r1 l2 r2.
+    (l1, r1) \<in> R \<longrightarrow> (l2, r2) \<in> R \<longrightarrow> (C1\<langle>l1\<rangle> = C2\<langle>l2\<rangle>) \<longrightarrow> ?q C1\<langle>r1\<rangle> C2\<langle>r2\<rangle>"
+  have "?p C12" for C12 :: "('f, string) ctxt \<times> ('f, string) ctxt"
+  proof -
+    let ?m = "[\<lambda>(C1, C2). size C1 + size C2, \<lambda> (C1, C2). size C1]"
+    show "?p C12"
+    proof (induct rule: wf_induct [OF wf_measures [of ?m], of ?p])
+      case (1 C12)
+      obtain C1 C2 where C12: "C12 = (C1, C2)" by force
+      show "?p C12" unfolding C12 split
+      proof (intro allI impI)
+        fix l1 r1 l2 r2
+        assume lr1: "(l1, r1) \<in> R" and lr2: "(l2, r2) \<in> R" and id: "C1\<langle>l1\<rangle> = C2\<langle>l2\<rangle>"
+        show "?q (C1\<langle>r1\<rangle>) (C2\<langle>r2\<rangle>)"
+        proof (cases C1)
+          case Hole note C1 = this
+          with id have id: "l1 = C2\<langle>l2\<rangle>" by simp
+          let ?p = "hole_pos C2"
+          show ?thesis
+          proof (cases "?p \<in> poss l1 \<and> is_Fun (l1 |_ ?p)")
+            case True
+            then have p: "?p \<in> poss l1" by auto
+            from ctxt_supt_id [OF p] obtain D where Dl1: "D\<langle>l1 |_ ?p\<rangle> = l1"
+              and D: "D = ctxt_of_pos_term (hole_pos C2) l1" by blast
+            from arg_cong [OF Dl1, of "\<lambda>t. t"]
+            have "(D)\<langle>(l1 |_ ?p)\<rangle> = C2\<langle>l2\<rangle>" unfolding id by simp
+            from arg_cong [OF this, of "\<lambda> t. t |_ ?p"]
+            have "l2 = (D)\<langle>(l1 |_ ?p)\<rangle> |_ ?p" by simp
+            also have "... = (D)\<langle>(l1 |_ ?p)\<rangle> |_ (hole_pos (D))"
+              using hole_pos_ctxt_of_pos_term [OF p] unfolding D by simp
+            also have "... = (l1 |_ ?p)" by (rule subt_at_hole_pos)
+            finally have ident: "l2 = l1 |_ ?p" by auto
+            have in_cp: "((D)\<langle>r2\<rangle>, r1) \<in> ground_critical_pairs R"
+              unfolding ground_critical_pairs_def mem_Collect_eq
+              by (metis Dl1 ident lr1 lr2)
+            from hole_pos_ctxt_of_pos_term [OF p] D have pD: "?p = hole_pos D" by simp
+            from id have C2: "C2 = ctxt_of_pos_term ?p (l1)" by simp
+            have "C2\<langle>r2\<rangle> = (ctxt_of_pos_term ?p (l1))\<langle>r2\<rangle>" using C2 by simp
+            also have "... = (D)\<langle>r2\<rangle>" unfolding D ..
+            finally have C2r\<sigma>: "C2\<langle>r2\<rangle> = D\<langle>r2\<rangle>" .
+            from C1 have C1r\<sigma>: "C1\<langle>r1\<rangle> = r1" by simp
+            show ?thesis unfolding C2r\<sigma> C1r\<sigma>
+            proof (rule disjI2, intro exI, intro conjI)
+              show "r1 = \<box>\<langle>r1\<rangle>" by simp
+            qed (insert in_cp, auto)
+          next
+            case False
+            hence False
+              using ground_R
+              using id lr1 vars_term_ctxt_apply by fastforce
+            thus ?thesis ..
+          qed
+        next
+          case (More f1 bef1 D1 aft1) note C1 = this
+          show ?thesis
+          proof (cases C2)
+            case Hole note C2 = this
+            from C1 C2 have "((C2, C1), C12) \<in> measures ?m" unfolding C12 by auto
+            from 1[rule_format, OF this, unfolded prod.case, rule_format, OF lr2 lr1 id[symmetric]]
+            show ?thesis
+            proof
+              assume "(C2\<langle>r2\<rangle>, C1\<langle>r1\<rangle>) \<in> join ?R"
+              then show ?thesis by auto
+            qed blast
+          next
+            case (More f2 bef2 D2 aft2) note C2 = this
+            let ?n1 = "length bef1"
+            let ?n2 = "length bef2"
+            note id = id [unfolded C1 C2]
+            from id have f: "f1 = f2" by simp
+            show ?thesis
+            proof (cases "?n1 = ?n2")
+              case True
+              with id have idb: "bef1 = bef2" and ida: "aft1 = aft2"
+                and idD: "D1\<langle>l1\<rangle> = D2\<langle>l2\<rangle>" by auto
+              let ?C = "More f2 bef2 \<box> aft2"
+              have id1: "C1 = ?C \<circ>\<^sub>c D1" unfolding C1 f ida idb by simp
+              have id2: "C2 = ?C \<circ>\<^sub>c D2" unfolding C2 by simp
+              have "((D1, D2), C12) \<in> measures ?m" unfolding C12 C1 C2
+                by auto
+              from 1 [rule_format, OF this, unfolded split, rule_format,
+                OF lr1 lr2 idD] have "?q (D1\<langle>r1\<rangle>) (D2\<langle>r2\<rangle>)" by auto
+              then show ?thesis
+              proof
+                assume "(D1\<langle>r1\<rangle>, D2\<langle>r2\<rangle>) \<in> join ?R"
+                then obtain s' where seq1: "(D1\<langle>r1\<rangle>, s') \<in> ?R^*"
+                and seq2: "(D2\<langle>r2\<rangle>, s') \<in> ?R^*" by auto
+                from rewrite_steps_closed_ctxt[OF seq1, of ?C]
+                have seq1: "(C1\<langle>r1\<rangle>, ?C\<langle>s'\<rangle>) \<in> ?R^*" unfolding id1 by simp
+                from rewrite_steps_closed_ctxt[OF seq2, of ?C]
+                have seq2: "(C2\<langle>r2\<rangle>, ?C\<langle>s'\<rangle>) \<in> ?R^*" using id2 by simp
+                from seq1 seq2 show ?thesis by auto
+              next
+                assume "\<exists>C l r. D1\<langle>r1\<rangle> = C\<langle>l\<rangle> \<and> D2\<langle>r2\<rangle> = C\<langle>r\<rangle> \<and> ((l, r) \<in> ?CP \<or> (r, l) \<in> ?CP)"
+                then obtain C l r where
+                  idD: "D1\<langle>r1\<rangle> = C\<langle>l\<rangle>" "D2\<langle>r2\<rangle> = C\<langle>r\<rangle>" and mem: "((l, r) \<in> ?CP \<or> (r, l) \<in> ?CP)"
+                  by blast
+                show ?thesis
+                  by (rule disjI2, unfold id1 id2, rule exI [of _ "?C \<circ>\<^sub>c C"], intro exI, rule conjI [OF _ conjI [OF _ mem]], insert idD, auto)
+              qed
+            next
+              case False
+              let ?p1 = "?n1 # hole_pos D1"
+              let ?p2 = "?n2 # hole_pos D2"
+              have l2: "C1\<langle>l1\<rangle> |_ ?p2 = l2 \<cdot> Var" unfolding C1 id by simp
+              have p12: "?p1  \<bottom> ?p2" using False by simp
+              have p1: "?p1 \<in> poss (C1\<langle>l1\<rangle>)" unfolding C1 by simp
+              have p2: "?p2 \<in> poss (C1\<langle>l1\<rangle>)" unfolding C1 unfolding id by simp
+              let ?one = "replace_at (C1\<langle>l1\<rangle>) ?p1 (r1)"
+              have one: "C1\<langle>r1\<rangle> = ?one" unfolding C1 by simp
+              have "(?one, replace_at ?one ?p2 (r2)) \<in> rewrite_steps R"
+                by (smt (verit, ccfv_threshold) CollectI ctxt_supt_id l2 lr2 p1 p12 p2
+                    parallel_poss_replace_at parallel_replace_at_subt_at rewrite_steps_def
+                    subst_apply_term_empty)
+              then have one: "(C1\<langle>r1\<rangle>, replace_at ?one ?p2 (r2)) \<in> (rewrite_steps R)^*" unfolding one by simp
+              have l1: "C2\<langle>l2\<rangle> |_ ?p1 = l1 \<cdot> Var" unfolding C2 id [symmetric] by simp
+              have p21: "?p2  \<bottom> ?p1" using False by simp
+              have p1': "?p1 \<in> poss (C2\<langle>l2\<rangle>)" unfolding C2 id [symmetric] by simp
+              have p2': "?p2 \<in> poss (C2\<langle>l2\<rangle>)" unfolding C2 by simp
+              let ?two = "replace_at (C2\<langle>l2\<rangle>) ?p2 (r2)"
+              have two: "C2\<langle>r2\<rangle> = ?two" unfolding C2 by simp
+              have "(?two, replace_at ?two ?p1 (r1)) \<in> rewrite_steps R"
+                by (smt (verit, ccfv_threshold) C1 CollectI More ctxt_supt_id id l1 lr1 p1 p2 p21
+                    parallel_poss_replace_at parallel_replace_at_subt_at rewrite_steps_def
+                    subst_apply_term_empty)
+              then have two: "(C2\<langle>r2\<rangle>, replace_at ?two ?p1 (r1)) \<in> (rewrite_steps R)^*" unfolding two by simp
+              have "replace_at ?one ?p2 (r2) = replace_at (replace_at (C1\<langle>l1\<rangle>) ?p2 (r2)) ?p1 (r1)"
+                by (rule parallel_replace_at [OF p12 p1 p2])
+              also have "... = replace_at ?two ?p1 (r1)" unfolding C1 C2 id ..
+              finally have one_two: "replace_at ?one ?p2 (r2) = replace_at ?two ?p1 (r1)" .
+              have "(C1\<langle>r1\<rangle>, C2\<langle>r2\<rangle>) \<in> (rewrite_steps R)\<^sup>\<down>"
+                using one one_two two by auto
+              thus ?thesis ..
+            qed
+          qed
+        qed
+      qed
+    qed
+  qed
+  from this[of "(C1, C2)", unfolded split, rule_format, OF lr1 lr2 id]
+  show ?thesis unfolding t1 t2 by auto
+qed
+
+lemma critical_pairs:
+  fixes R :: "('f, string) trs"
+  assumes ground_R: "\<forall>(s, t) \<in> R. is_ground_trm s \<and> is_ground_trm t"
+  assumes cp: "\<And> l r. (l, r) \<in> ground_critical_pairs R \<Longrightarrow> l \<noteq> r \<Longrightarrow>
+    \<exists>s. (l, s) \<in> (rewrite_steps R)\<^sup>* \<and> (r, s) \<in> (rewrite_steps R)\<^sup>*"
+  shows "WCR (rewrite_steps R)"
+proof (rule WCR_onI)
+  let ?R = "rewrite_steps R"
+  let ?CP = "ground_critical_pairs R"
+  fix s t1 t2
+  assume steps: "(s, t1) \<in> ?R" "(s, t2) \<in> ?R"
+  let ?p = "\<lambda> s'. (t1, s') \<in> ?R^* \<and> (t2, s') \<in> ?R^*"
+  from critical_pairs_main [OF ground_R steps]
+  have "\<exists> s'. ?p s'"
+  proof (elim disjE)
+    assume "\<exists>ctxt l r. t1 = ctxt\<langle>l\<rangle> \<and> t2 = ctxt\<langle>r\<rangle> \<and> ((l, r) \<in> ?CP \<or> (r, l) \<in> ?CP)"
+    then obtain C l r where id: "t1 = C\<langle>l\<rangle>" "t2 = C\<langle>r\<rangle>"
+      and mem: "(l, r) \<in> ?CP \<or> (r, l) \<in> ?CP" by blast
+    show ?thesis
+    proof (cases "l = r")
+      case True
+      then show ?thesis unfolding id by auto
+    next
+      case False
+      from mem show ?thesis
+      proof (elim disjE)
+        assume mem: "(l, r) \<in> ?CP"
+        show "\<exists> s'. ?p s'"
+          using cp[OF mem False] id rewrite_steps_closed_ctxt by blast
+      next
+        assume mem: "(r, l) \<in> ?CP"
+        show "\<exists> s'. ?p s'"
+          using cp[OF mem] id rewrite_steps_closed_ctxt by blast
+      qed
+    qed
+  qed auto
+  thus "(t1, t2) \<in> join ?R" by auto
+qed
+
+lemma critical_pair_lemma:
+  fixes R :: "('f, string) trs"
+  assumes ground_R: "\<forall>(s, t) \<in> R. is_ground_trm s \<and> is_ground_trm t"
+  shows "WCR (rewrite_steps R) \<longleftrightarrow>
+    (\<forall>(s, t) \<in> ground_critical_pairs R. (s, t) \<in> (rewrite_steps R)\<^sup>\<down>)"
+  (is "?l = ?r")
+proof
+  assume "WCR (rewrite_steps R)"
+  thus "\<forall>(s, t) \<in> ground_critical_pairs R. (s, t) \<in> (rewrite_steps R)\<^sup>\<down>"
+    using ground_critical_pairs_complete by blast
+next
+  assume all_cp_joinable: "\<forall>(s, t) \<in> ground_critical_pairs R. (s, t) \<in> (rewrite_steps R)\<^sup>\<down>"
+  show "WCR (rewrite_steps R)"
+  proof (rule critical_pairs[OF ground_R])
+    fix s t
+    assume "(s, t) \<in> ground_critical_pairs R"
+    with all_cp_joinable have "(s, t) \<in> join (rewrite_steps R)" by auto
+    then obtain u where s: "(s, u) \<in> (rewrite_steps R)^*"
+      and t: "(t, u) \<in> (rewrite_steps R)^*" by auto
+    thus "\<exists>u. (s, u) \<in> (rewrite_steps R)^* \<and> (t, u) \<in> (rewrite_steps R)^*"
+      by metis
+  qed
+qed
+
+(* lemma ground_critical_pair_lemma:
+  fixes R :: "('f, string) trs"
+  assumes ground_R: "\<forall>(s, t) \<in> R. is_ground_trm s \<and> is_ground_trm t"
+  shows "WCR (rewrite_steps R) \<longleftrightarrow> (\<forall> (s, t) \<in> ground_critical_pairs R. (s, t) \<in> (rewrite_steps R)\<^sup>\<down>)"
+  using critical_pair_lemma[OF ground_R]
   using mem_critical_pairs_if_mem_ground_critical_pairs[OF ground_R]
-  using mem_ground_critical_pairs_if_mem_critical_pairs[OF ground_R]
-  by (metis (no_types, lifting) case_prodD case_prodI2)
+  using mem_ground_critical_pairs_if_mem_critical_pairs[OF ground_R] *)
+  (* by (metis (no_types, lifting) case_prodD case_prodI2) *)
 
 global_interpretation ground_critical_pair_lemma "undefined :: 'f" "undefined :: string"
 proof unfold_locales
   fix R :: "('f, string) trs"
-  assume "vars_trs R = {}"
+  assume "(\<Union>r \<in> R. vars_rewrite_rule r)= {}"
   hence ground_R: "\<forall>(s, t)\<in>R. is_ground_trm s \<and> is_ground_trm t"
-    by (auto simp add: vars_trs_def vars_rule_def)
-  show "WCR (rstep R) = (ground_critical_pairs R \<subseteq> (rstep R)\<^sup>\<down>)"
-    using ground_critical_pair_lemma[OF ground_R] by auto
+    by (auto simp: vars_rewrite_rule_def)
+  show "WCR (rewrite_steps R) = (ground_critical_pairs R \<subseteq> (rewrite_steps R)\<^sup>\<down>)"
+    using critical_pair_lemma[OF ground_R] by auto
 qed
 
 end
